theories/Analysis/DomainSSA.v
@@ -1,0 +1,125 @@
+Require Import CSet Le CMap CMapDomain CMapPartialOrder CMapJoinSemiLattice CMapTerminating.
+
+Require Import Plus Util AllInRel CSet OptionR.
+Require Import Val Var Env IL Annotation Infra.Lattice DecSolve.
+Require Import CMap WithTop.
+Require Import MapNotations ListUpdateAt.
+Require Import Terminating OptionR.
+
+Set Implicit Arguments.
+
+Open Scope map_scope.
+
+Definition Dom D := Map [var, D].
+
+Definition domupd D (d:Dom D) x (o:option D) : Dom D :=
+  match o with
+  | Some xv => (d [- x <- xv -])
+  | None => remove x d
+  end.
+
+Fixpoint domjoin_list D `{JoinSemiLattice D} (m:Dom D) (A:list var) (B:list (option D)) :=
+  match A, B with
+  | x::A, y::B =>
+    domupd (domjoin_list m A B) x (join (find x m) y)
+  | _, _ => m
+  end.
+
+Definition domenv D (d:Dom D) (x:var) : option D :=
+  find x d.
+
+Lemma poLe_option_None X `{PartialOrder X} (x:option X)
+  :  ⎣⎦ ⊑ x.
+Proof.
+  econstructor.
+Qed.
+
+Hint Resolve poLe_option_None.
+
+Lemma domupd_le D `{PartialOrder D} (a b: Dom D) v v' x
+  : leMap a b
+    -> poLe v v'
+    -> leMap (domupd a x v) (domupd b x v').
+Proof.
+  unfold leMap, domupd; intros.
+  inv H1.
+  - repeat cases; clear_trivial_eqs; mlud; eauto.
+  - mlud; eauto.
+Qed.
+
+Lemma domjoin_list_le D `{JoinSemiLattice D} (a b: Dom D) Z Y Y'
+  : leMap a b
+    -> poLe Y Y'
+    -> leMap (domjoin_list a Z Y)
+            (domjoin_list b Z Y').
+Proof.
+  general induction Z; simpl domjoin_list; eauto.
+  inv H2; eauto.
+  - eapply domupd_le.
+    + eapply IHZ; eauto.
+    + eapply ojoin_poLe; eauto.
+Qed.
+
+Lemma domupd_eq D `{PartialOrder D} (a b: Dom D) v v' x
+  : eqMap a b
+    -> poEq v v'
+    -> eqMap (domupd a x v) (domupd b x v').
+Proof.
+  unfold eqMap, domupd; intros.
+  inv H1.
+  - eapply eqMap_remove; eauto.
+  - repeat cases; clear_trivial_eqs. mlud; eauto.
+    econstructor. eauto.
+Qed.
+
+Lemma domjoin_list_eq  D `{JoinSemiLattice D} (a b: Dom D) Z Y Y'
+  : eqMap a b
+    -> poEq Y Y'
+    -> eqMap (domjoin_list a Z Y)
+            (domjoin_list b Z Y').
+Proof.
+  general induction Z; simpl domjoin_list; eauto.
+  inv H2; eauto.
+  - eapply domupd_eq
+    + eapply IHZ; eauto.
+    + eapply ojoin_poEq; eauto.
+Qed.
+
+Lemma domjoin_ne D `{JoinSemiLattice D} (m:Dom D) x y a
+  : x =/= y
+    -> find x (domupd m y a) = find x m.
+Proof.
+  unfold domupd; cases; intros; mlud; eauto.
+Qed.
+
+Lemma domjoin_list_ne D `{JoinSemiLattice D} (m:Dom D) x Z Y
+  : ~ InA eq x Z
+    -> find x (domjoin_list m Z Y) === find x m.
+Proof.
+  intros NI.
+  general induction Z; destruct Y; simpl; eauto.
+  erewrite domjoin_ne; eauto. eapply IHZ; eauto.
+  intro; eapply NI; econstructor. eapply H1.
+Qed.
+
+Lemma domjoin_list_exp  D `{JoinSemiLattice D} (m:Dom D) Z Y
+  : leMap m (domjoin_list m Z Y).
+Proof.
+  general induction Z; destruct Y; simpl domjoin_list; eauto;
+    try reflexivity.
+  unfold ojoin; repeat cases; simpl domupd; eauto.
+  - hnf; intros. mlud.
+    + rewrite <- e, <- Heq.
+      econstructor.
+      eapply join_poLe.
+    + eapply IHZ.
+  - hnf; intros; mlud.
+    rewrite Heq, e; eauto.
+    eapply IHZ.
+  - hnf; intros; mlud.
+    rewrite <- e, <- Heq; eauto.
+    eapply IHZ.
+  - hnf; intros; mlud.
+    rewrite <- e, <- Heq; eauto.
+    eapply IHZ.
+Qed.
